AVL tree overhaul to remove LargeAlloc assumes
remaining:
- one sl-related admit (coercion...) still!
- one assume in lib_avl_common/ to be removed
- two sladmit to be removed
- one admit, some work ahead with precondition
propagation

lib_avl_common/Impl.Core.fst
@@ -12,15 +12,14 @@ module Spec = Spec.Trees
 
 #set-options "--fuel 1 --ifuel 1 --z3rlimit 15"
 
-#push-options "--__no_positivity"
-noeq type node (a: Type0) = {
+noeq
+type node (a: Type0) = {
   data: a;
   left: ref (node a);
   right: ref (node a);
   size: U.t;
   height: U.t;
 }
-#pop-options
 
 let get_left #a n = n.left
 let get_right #a n = n.right
@@ -39,18 +38,20 @@ let mk_node #a data left right size height = {
 let null_t #a = null
 let is_null_t #a ptr = is_null ptr
 
-let rec tree_sl' (#a: Type0) (ptr: t a) (tree: wdm (node a))
+let rec tree_sl' (#a: Type0) (p: hpred a) (ptr: t a) (tree: wdm (node a))
   : Tot slprop (decreases tree)
   =
   match tree with
   | Spec.Leaf -> Mem.pure (ptr == null_t)
   | Spec.Node data left right size height ->
     pts_to_sl ptr full_perm data `Mem.star`
-    tree_sl' (get_left data) left `Mem.star`
-    tree_sl' (get_right data) right `Mem.star`
-    Mem.pure (get_size data == U.uint_to_t size /\ get_height data == U.uint_to_t height)
+    tree_sl' p (get_left data) left `Mem.star`
+    tree_sl' p (get_right data) right `Mem.star`
+    Mem.pure (get_size data == U.uint_to_t size /\ get_height data == U.uint_to_t height) `Mem.star`
+    Mem.pure ((G.reveal p) (get_left data) /\
+              (G.reveal p) (get_right data))
 
-let tree_sl #a ptr = Mem.h_exists (tree_sl' ptr)
+let tree_sl #a p ptr = Mem.h_exists (tree_sl' p ptr)
 
 let rec tree_view_aux (#a: Type0) (tree: wdm (node a))
   : Tot (Spec.tree a) (decreases tree)
@@ -101,22 +102,24 @@ let tree_view (#a: Type0) (tree: wdm (node a))
   tree_view_aux_same_size2 tree;
   tree_view_aux tree
 
-let tree_sel_node' (#a: Type0) (ptr: t a) : selector' (wdm (node a)) (tree_sl ptr) =
-  fun h -> id_elim_exists (tree_sl' ptr) h
+let tree_sel_node' (#a: Type0) (p: hpred a) (ptr: t a) : selector' (wdm (node a)) (tree_sl p ptr) =
+  fun h -> id_elim_exists (tree_sl' p ptr) h
 
-let tree_sl'_witinv (#a: Type0) (ptr: t a) : Lemma(is_witness_invariant (tree_sl' ptr))
-  = let rec aux (ptr:t a) (x y:wdm (node a)) (m:mem) : Lemma
-        (requires interp (tree_sl' ptr x) m /\ interp (tree_sl' ptr y) m)
-        (ensures x == y)
-        (decreases x)
+let tree_sl'_witinv (#a: Type0) (p: hpred a) (ptr: t a)
+  : Lemma(is_witness_invariant (tree_sl' p ptr))
+  = let rec aux (ptr:t a) (x y:wdm (node a)) (m:mem)
+    : Lemma
+    (requires interp (tree_sl' p ptr x) m /\ interp (tree_sl' p ptr y) m)
+    (ensures x == y)
+    (decreases x)
     = match x with
       | Spec.Leaf -> begin match y with
          | Spec.Leaf -> ()
          | Spec.Node data left right size height ->
            Mem.pure_interp (ptr == null_t) m;
            let p1 = pts_to_sl ptr full_perm data in
-           let p2 = tree_sl' (get_left data) left in
-           let p3 = tree_sl' (get_right data) right in
+           let p2 = tree_sl' p (get_left data) left in
+           let p3 = tree_sl' p (get_right data) right in
            let p4 = Mem.pure (get_size data == U.uint_to_t size) in
            let p5 = Mem.pure (get_height data == U.uint_to_t height) in
            Mem.affine_star (p1 `Mem.star` p2 `Mem.star` p3 `Mem.star` p4) p5 m;
@@ -129,8 +132,8 @@ let tree_sl'_witinv (#a: Type0) (ptr: t a) : Lemma(is_witness_invariant (tree_sl
         | Spec.Leaf ->
            Mem.pure_interp (ptr == null_t) m;
            let p1 = pts_to_sl ptr full_perm data1 in
-           let p2 = tree_sl' (get_left data1) left1 in
-           let p3 = tree_sl' (get_right data1) right1 in
+           let p2 = tree_sl' p (get_left data1) left1 in
+           let p3 = tree_sl' p (get_right data1) right1 in
            let p4 = Mem.pure (get_size data1 == U.uint_to_t size1) in
            let p5 = Mem.pure (get_height data1 == U.uint_to_t height1) in
            Mem.affine_star (p1 `Mem.star` p2 `Mem.star` p3 `Mem.star` p4) p5 m;
@@ -155,130 +158,133 @@ let tree_sl'_witinv (#a: Type0) (ptr: t a) : Lemma(is_witness_invariant (tree_sl
     in
     Classical.forall_intro_3 (Classical.move_requires_3 (aux ptr))
 
-let tree_sel_depends_only_on (#a:Type0) (ptr:t a)
-  (m0:Mem.hmem (tree_sl ptr)) (m1:mem{disjoint m0 m1})
-  : Lemma (tree_sel_node' ptr m0 == tree_sel_node' ptr (Mem.join m0 m1))
+let tree_sel_depends_only_on (#a:Type0) (p: hpred a) (ptr:t a)
+  (m0:Mem.hmem (tree_sl p ptr)) (m1:mem{disjoint m0 m1})
+  : Lemma (tree_sel_node' p ptr m0 == tree_sel_node' p ptr (Mem.join m0 m1))
   =
-  let m':Mem.hmem (tree_sl ptr) = Mem.join m0 m1 in
-  let t1 = Ghost.reveal (id_elim_exists (tree_sl' ptr) m0) in
-  let t2 = Ghost.reveal (id_elim_exists (tree_sl' ptr) m') in
-  tree_sl'_witinv ptr;
-  Mem.elim_wi (tree_sl' ptr) t1 t2 m'
+  let m':Mem.hmem (tree_sl p ptr) = Mem.join m0 m1 in
+  let t1 = Ghost.reveal (id_elim_exists (tree_sl' p ptr) m0) in
+  let t2 = Ghost.reveal (id_elim_exists (tree_sl' p ptr) m') in
+  tree_sl'_witinv p ptr;
+  Mem.elim_wi (tree_sl' p ptr) t1 t2 m'
 
-let tree_sel_depends_only_on_core (#a:Type0) (ptr:t a)
-  (m0:Mem.hmem (tree_sl ptr))
-  : Lemma (tree_sel_node' ptr m0 == tree_sel_node' ptr (core_mem m0))
+let tree_sel_depends_only_on_core (#a:Type0) (p: hpred a) (ptr:t a)
+  (m0:Mem.hmem (tree_sl p ptr))
+  : Lemma (tree_sel_node' p ptr m0 == tree_sel_node' p ptr (core_mem m0))
   =
-  let t1 = Ghost.reveal (id_elim_exists (tree_sl' ptr) m0) in
-  let t2 = Ghost.reveal (id_elim_exists (tree_sl' ptr) (core_mem m0)) in
-  tree_sl'_witinv ptr;
-  Mem.elim_wi (tree_sl' ptr) t1 t2 (core_mem m0)
+  let t1 = Ghost.reveal (id_elim_exists (tree_sl' p ptr) m0) in
+  let t2 = Ghost.reveal (id_elim_exists (tree_sl' p ptr) (core_mem m0)) in
+  tree_sl'_witinv p ptr;
+  Mem.elim_wi (tree_sl' p ptr) t1 t2 (core_mem m0)
 
-let tree_sel_node (#a: Type0) (ptr: t a) : selector (wdm (node a)) (tree_sl ptr) =
-  Classical.forall_intro_2 (tree_sel_depends_only_on ptr);
-  Classical.forall_intro (tree_sel_depends_only_on_core ptr);
-  tree_sel_node' ptr
+let tree_sel_node (#a: Type0) (p: hpred a) (ptr: t a)
+  : selector (wdm (node a)) (tree_sl p ptr) =
+  Classical.forall_intro_2 (tree_sel_depends_only_on p ptr);
+  Classical.forall_intro (tree_sel_depends_only_on_core p ptr);
+  tree_sel_node' p ptr
 
-let tree_sel #a r =
-  fun h -> tree_view (tree_sel_node r h)
+let tree_sel #a p r =
+  fun h -> tree_view (tree_sel_node p r h)
 
-let tree_sel_interp (#a: Type0) (ptr: t a) (t: wdm (node a)) (m: mem) : Lemma
-  (requires interp (tree_sl' ptr t) m)
-  (ensures interp (tree_sl ptr) m /\ tree_sel_node' ptr m == t)
-  = intro_h_exists t (tree_sl' ptr) m;
-    tree_sl'_witinv ptr
+let tree_sel_interp (#a: Type0) (p: hpred a) (ptr: t a) (t: wdm (node a)) (m: mem)
+  : Lemma
+  (requires interp (tree_sl' p ptr t) m)
+  (ensures interp (tree_sl p ptr) m /\ tree_sel_node' p ptr m == t)
+  = intro_h_exists t (tree_sl' p ptr) m;
+    tree_sl'_witinv p ptr
 
-let intro_leaf_lemma (a:Type0) (m:mem) : Lemma
+let intro_leaf_lemma (a:Type0) (p: hpred a) (m:mem) : Lemma
     (requires interp (hp_of emp) m)
-    (ensures interp (tree_sl (null_t #a)) m /\ tree_sel (null_t #a) m == Spec.Leaf)
+    (ensures interp (tree_sl p (null_t #a)) m /\ tree_sel p (null_t #a) m == Spec.Leaf)
     = let ptr:t a = null_t in
       pure_interp (ptr == null_t) m;
       let open FStar.Tactics in
-      assert (tree_sl' ptr Spec.Leaf == Mem.pure (ptr == null_t)) by (norm [delta; zeta; iota]);
-      tree_sel_interp ptr Spec.Leaf m
+      assert (tree_sl' p ptr Spec.Leaf == Mem.pure (ptr == null_t)) by (norm [delta; zeta; iota]);
+      tree_sel_interp p ptr Spec.Leaf m
 
-let intro_linked_tree_leaf #opened #a _ =
-    change_slprop_2 emp (linked_tree (null_t #a)) (Spec.Leaf <: wdm a) (intro_leaf_lemma a)
+let intro_linked_tree_leaf #opened #a p _ =
+    change_slprop_2 emp (linked_tree p (null_t #a)) (Spec.Leaf <: wdm a) (intro_leaf_lemma a p)
 
-let elim_leaf_lemma (#a:Type0) (ptr:t a) (m:mem) : Lemma
-    (requires interp (tree_sl ptr) m /\ ptr == null_t)
-    (ensures interp (hp_of emp) m /\ tree_sel ptr m == Spec.Leaf)
-    = let l' = id_elim_exists (tree_sl' ptr) m in
+let elim_leaf_lemma (#a:Type0) (p: hpred a) (ptr:t a) (m:mem) : Lemma
+    (requires interp (tree_sl p ptr) m /\ ptr == null_t)
+    (ensures interp (hp_of emp) m /\ tree_sel p ptr m == Spec.Leaf)
+    = let l' = id_elim_exists (tree_sl' p ptr) m in
       pure_interp (ptr == null_t) m;
-      tree_sel_interp ptr Spec.Leaf m;
+      tree_sel_interp p ptr Spec.Leaf m;
       reveal_emp ();
       intro_emp m
 
-let elim_linked_tree_leaf #opened #a ptr =
-  change_slprop_rel (linked_tree ptr) emp
+let elim_linked_tree_leaf #opened #a p ptr =
+  change_slprop_rel (linked_tree p ptr) emp
     (fun x y -> x == Spec.Leaf)
-    (fun m -> elim_leaf_lemma ptr m)
+    (fun m -> elim_leaf_lemma p ptr m)
 
-
-let lemma_node_is_not_null (#a:Type) (ptr:t a) (t:wdm a) (m:mem) : Lemma
-    (requires interp (tree_sl ptr) m /\ tree_sel ptr m == t /\ Spec.Node? t)
+let lemma_node_is_not_null (#a:Type) (p: hpred a) (ptr:t a) (t:wdm a) (m:mem) : Lemma
+    (requires interp (tree_sl p ptr) m /\ tree_sel p ptr m == t /\ Spec.Node? t)
     (ensures ptr =!= null_t)
     =
-      let t':wdm (node a) = id_elim_exists (tree_sl' ptr) m in
-      assert (interp (tree_sl' ptr t') m);
-      tree_sel_interp ptr t' m;
+      let t':wdm (node a) = id_elim_exists (tree_sl' p ptr) m in
+      assert (interp (tree_sl' p ptr t') m);
+      tree_sel_interp p ptr t' m;
       match reveal t' with
       | Spec.Node data _ _ _ _ ->
            pts_to_not_null ptr full_perm data m
 
-let lemma_not_null_is_node (#a:Type) (ptr:t a) (t:wdm a) (m:mem) : Lemma
-  (requires interp (tree_sl ptr) m /\ tree_sel ptr m == t /\ ptr =!= null_t)
+let lemma_not_null_is_node (#a:Type) (p: hpred a) (ptr:t a) (t:wdm a) (m:mem) : Lemma
+  (requires interp (tree_sl p ptr) m /\ tree_sel p ptr m == t /\ ptr =!= null_t)
   (ensures Spec.Node? t)
   =
-  let t': wdm (node a) = id_elim_exists (tree_sl' ptr) m in
-  assert (interp (tree_sl' ptr t') m);
-  tree_sel_interp ptr t' m;
+  let t': wdm (node a) = id_elim_exists (tree_sl' p ptr) m in
+  assert (interp (tree_sl' p ptr t') m);
+  tree_sel_interp p ptr t' m;
   match reveal t' with
   | Spec.Leaf -> Mem.pure_interp (ptr == null_t) m
   | _ -> ()
 
-let null_is_leaf #opened #a ptr =
-  change_slprop_rel (linked_tree ptr) (linked_tree ptr)
+let null_is_leaf #opened #a p ptr =
+  change_slprop_rel (linked_tree p ptr) (linked_tree p ptr)
     (fun x y -> x == y /\ y == Spec.Leaf)
-    (fun m -> elim_leaf_lemma ptr m)
+    (fun m -> elim_leaf_lemma p ptr m)
 
-let lemma_leaf_is_null (#a:Type) (ptr:t a) (t:wdm a) (m:mem) : Lemma
-  (requires interp (tree_sl ptr) m /\ tree_sel ptr m == t /\
+let lemma_leaf_is_null (#a:Type) (p: hpred a) (ptr:t a) (t:wdm a) (m:mem) : Lemma
+  (requires interp (tree_sl p ptr) m /\ tree_sel p ptr m == t /\
     Spec.Leaf? t)
   (ensures ptr == null_t)
   =
-  let t':wdm (node a) = id_elim_exists (tree_sl' ptr) m in
-  assert (interp (tree_sl' ptr t') m);
-  tree_sel_interp ptr t' m;
+  let t':wdm (node a) = id_elim_exists (tree_sl' p ptr) m in
+  assert (interp (tree_sl' p ptr t') m);
+  tree_sel_interp p ptr t' m;
   match reveal t' with
   | Spec.Leaf -> Mem.pure_interp (ptr == null_t) m
   | _ -> ()
 
-let leaf_is_null #opened #a ptr =
+let leaf_is_null #opened #a p ptr =
   let h = get () in
-  let t : erased (wdm a) = hide (v_linked_tree ptr h) in
-  extract_info (linked_tree ptr) t (ptr == null_t)
-    (lemma_leaf_is_null ptr t)
+  let t : erased (wdm a) = hide (v_linked_tree p ptr h) in
+  extract_info (linked_tree p ptr) t (ptr == null_t)
+    (lemma_leaf_is_null p ptr t)
 
-let node_is_not_null #opened #a ptr =
+let node_is_not_null #opened #a p ptr =
   let h = get () in
-  let t : erased (wdm a) = hide (v_linked_tree ptr h) in
-  extract_info (linked_tree ptr) t (ptr =!= null_t) (lemma_node_is_not_null ptr t)
+  let t : erased (wdm a) = hide (v_linked_tree p ptr h) in
+  extract_info (linked_tree p ptr) t (ptr =!= null_t) (lemma_node_is_not_null p ptr t)
 
-let not_null_is_node #opened #a ptr =
+let not_null_is_node #opened #a p ptr =
   let h = get () in
-  let t : erased (wdm a) = hide (v_linked_tree ptr h) in
-  extract_info (linked_tree ptr) t (Spec.Node? t == true) (lemma_not_null_is_node ptr t)
+  let t : erased (wdm a) = hide (v_linked_tree p ptr h) in
+  extract_info (linked_tree p ptr) t (Spec.Node? t == true) (lemma_not_null_is_node p ptr t)
 
-let pack_tree_lemma_aux (#a:Type0) (pt:t a)
+let pack_tree_lemma_aux (#a:Type0) (p: hpred a) (pt:t a)
   (x: node a) (l r: wdm (node a)) (s h:nat) (m:mem) : Lemma
   (requires
     s <= c /\
     h <= c /\
     interp (pts_to_sl pt full_perm x `Mem.star`
-      tree_sl' (get_left x) l `Mem.star`
-      tree_sl' (get_right x) r `Mem.star`
-      Mem.pure (get_size x == U.uint_to_t s /\ get_height x == U.uint_to_t h)
+      tree_sl' p (get_left x) l `Mem.star`
+      tree_sl' p (get_right x) r `Mem.star`
+      Mem.pure (get_size x == U.uint_to_t s /\ get_height x == U.uint_to_t h) `Mem.star`
+      Mem.pure ((G.reveal p) (get_left x) /\
+                (G.reveal p) (get_right x))
       ) m
     /\ s = Spec.size_of_tree l + Spec.size_of_tree r + 1
     /\ h = M.max (Spec.height_of_tree l) (Spec.height_of_tree r) + 1
@@ -289,7 +295,7 @@ let pack_tree_lemma_aux (#a:Type0) (pt:t a)
      //let s = Spec.size_of_tree l + Spec.size_of_tree r + 1 in
      let t = Spec.Node x l r s h in
      // let t: wds (node a) = t in
-     interp (tree_sl' pt t) m))
+     interp (tree_sl' p pt t) m))
   =
     //let s = Spec.size_of_tree l + Spec.size_of_tree r + 1 in
     let t = Spec.Node x l r s h in
@@ -318,15 +324,16 @@ let pack_tree_lemma_aux (#a:Type0) (pt:t a)
       m
 *)
 
+#push-options "--z3rlimit 30"
 // Maintenant, tenter en ajoutant s (et sr) en paramètre(s)
-let pack_tree_lemma (#a:Type0) (pt left right:t a) (sr hr: U.t)
+let pack_tree_lemma (#a:Type0) (p: hpred a) (pt left right:t a) (sr hr: U.t)
   (x: node a) (l r:wdm a) (s h:nat) (m:mem) : Lemma
   (requires
     s <= c /\
     h <= c /\
     interp (ptr pt `Mem.star`
-      tree_sl left `Mem.star`
-      tree_sl right) m /\
+      tree_sl p left `Mem.star`
+      tree_sl p right) m /\
     get_left x == left /\
     get_right x == right /\
     get_size x == sr /\
@@ -334,10 +341,12 @@ let pack_tree_lemma (#a:Type0) (pt left right:t a) (sr hr: U.t)
     sel_of (vptr pt) m == x /\
     U.v sr == s /\
     U.v hr == h /\
-    sel_of (linked_tree left) m == l /\
-    sel_of (linked_tree right) m == r /\
+    sel_of (linked_tree p left) m == l /\
+    sel_of (linked_tree p right) m == r /\
     s == Spec.size_of_tree l + Spec.size_of_tree r + 1 /\
-    h == M.max (Spec.height_of_tree l) (Spec.height_of_tree r) + 1
+    h == M.max (Spec.height_of_tree l) (Spec.height_of_tree r) + 1 /\
+    (G.reveal p) (get_left x) /\
+    (G.reveal p) (get_right x)
   )
   (ensures
     (
@@ -345,52 +354,59 @@ let pack_tree_lemma (#a:Type0) (pt left right:t a) (sr hr: U.t)
     assert (Spec.is_wdm l);
     assert (Spec.is_wdm r);
     assert (Spec.is_wdm t);
-    interp (tree_sl pt) m /\
-    tree_sel pt m == Spec.Node (get_data x) l r s h)
+    interp (tree_sl p pt) m /\
+    tree_sel p pt m == Spec.Node (get_data x) l r s h)
   )
   =
     let t = Spec.Node (get_data x) l r s h in
     assert (Spec.is_wdm t);
 
-    let l':wdm (node a) = id_elim_exists (tree_sl' left) m in
-    let r':wdm (node a) = id_elim_exists (tree_sl' right) m in
+    let l':wdm (node a) = id_elim_exists (tree_sl' p left) m in
+    let r':wdm (node a) = id_elim_exists (tree_sl' p right) m in
     let p1 = ptr pt in
-    let p2 = tree_sl left in
-    let p3 = tree_sl right in
+    let p2 = tree_sl p left in
+    let p3 = tree_sl p right in
     let m12, m3 = id_elim_star (p1 `Mem.star` p2) p3 m in
     let m1, m2 = id_elim_star p1 p2 m12 in
     //assert (ptr_sel sr m == s);
     // #1
     ptr_sel_interp pt m1;
     // #2
-    let l2:wdm (node a) = id_elim_exists (tree_sl' left) m2 in
+    let l2:wdm (node a) = id_elim_exists (tree_sl' p left) m2 in
     join_commutative m1 m2;
-    assert (interp (tree_sl' left l2) m);
-    tree_sl'_witinv left;
+    assert (interp (tree_sl' p left l2) m);
+    tree_sl'_witinv p left;
     assert (l2 == l');
-    assert (interp (tree_sl' left l') m2);
+    assert (interp (tree_sl' p left l') m2);
     // #3
-    let r2:wdm (node a) = id_elim_exists (tree_sl' right) m3 in
+    let r2:wdm (node a) = id_elim_exists (tree_sl' p right) m3 in
     join_commutative m12 m3;
-    assert (interp (tree_sl' right r2) m);
-    tree_sl'_witinv right;
+    assert (interp (tree_sl' p right r2) m);
+    tree_sl'_witinv p right;
     assert (r2 == r');
-    assert (interp (tree_sl' right r') m3);
+    assert (interp (tree_sl' p right r') m3);
 
-    intro_star (pts_to_sl pt full_perm x) (tree_sl' left l') m1 m2;
+    intro_star (pts_to_sl pt full_perm x) (tree_sl' p left l') m1 m2;
     intro_star
-      (pts_to_sl pt full_perm x `Mem.star` tree_sl' left l')
-      (tree_sl' right r')
+      (pts_to_sl pt full_perm x `Mem.star` tree_sl' p left l')
+      (tree_sl' p right r')
       m12 m3;
     Mem.emp_unit (pts_to_sl pt full_perm x `Mem.star`
-      tree_sl' left l' `Mem.star`
-      tree_sl' right r'
+      tree_sl' p left l' `Mem.star`
+      tree_sl' p right r'
       );
     Mem.pure_star_interp (pts_to_sl pt full_perm x `Mem.star`
-      tree_sl' left l' `Mem.star`
-      tree_sl' right r'
+      tree_sl' p left l' `Mem.star`
+      tree_sl' p right r'
       )
       (get_size x == U.uint_to_t s /\ get_height x == U.uint_to_t h)
+      m;
+    Mem.pure_star_interp (pts_to_sl pt full_perm x `Mem.star`
+      tree_sl' p left l' `Mem.star`
+      tree_sl' p right r' `Mem.star`
+      Mem.pure (get_size x == U.uint_to_t s /\ get_height x == U.uint_to_t h)
+      )
+      ((G.reveal p) (get_left x) /\ (G.reveal p) (get_right x))
       m;
 
 
@@ -398,55 +414,66 @@ let pack_tree_lemma (#a:Type0) (pt left right:t a) (sr hr: U.t)
     let h = M.max (Spec.height_of_tree l') (Spec.height_of_tree r') + 1 in
     let t = Spec.Node x l' r' s h in
 
-    pack_tree_lemma_aux pt x l' r' s h m;
-    intro_h_exists t (tree_sl' pt) m;
-    tree_sel_interp pt t m
+    assume (interp (pts_to_sl pt full_perm x `Mem.star`
+      tree_sl' p (get_left x) l' `Mem.star`
+      tree_sl' p (get_right x) r' `Mem.star`
+      Mem.pure (get_size x == U.uint_to_t s /\ get_height x == U.uint_to_t h) `Mem.star`
+      Mem.pure ((G.reveal p) (get_left x) /\
+                (G.reveal p) (get_right x))
+      ) m
+    );
 
-let pack_tree #opened #a ptr left right sr hr =
+    pack_tree_lemma_aux p pt x l' r' s h m;
+    intro_h_exists t (tree_sl' p pt) m;
+    tree_sel_interp p pt t m
+#pop-options
+
+let pack_tree #opened #a p ptr left right sr hr =
   let h0 = get () in
   let x = hide (sel ptr h0) in
-  let l:wdm a = hide (v_linked_tree left h0) in
-  let r:wdm a = hide (v_linked_tree right h0) in
+  let l:wdm a = hide (v_linked_tree p left h0) in
+  let r:wdm a = hide (v_linked_tree p right h0) in
   let t = Spec.Node (get_data x) l r (U.v sr) (U.v hr) in
 
   change_slprop
     (vptr ptr `star`
-    linked_tree left `star`
-    linked_tree right)
-    (linked_tree ptr)
+    linked_tree p left `star`
+    linked_tree p right)
+    (linked_tree p ptr)
     ((reveal x, reveal l), reveal r) t
-    (fun m -> pack_tree_lemma ptr left right sr hr x l r (U.v sr) (U.v hr) m)
+    (fun m -> pack_tree_lemma p ptr left right sr hr x l r (U.v sr) (U.v hr) m)
 
 [@@__steel_reduce__]
-let tree_node' #a r : vprop' =
-  {hp = tree_sl r;
+let tree_node' #a p r : vprop' =
+  {hp = tree_sl p r;
    t = wdm (node a);
-   sel = tree_sel_node r}
+   sel = tree_sel_node p r}
 unfold
-let tree_node (#a:Type0) (r:t a) = VUnit (tree_node' r)
+let tree_node (#a:Type0) p (r:t a) = VUnit (tree_node' p r)
 
 [@@ __steel_reduce__]
 let v_node
   (#a:Type0)
-  (#p:vprop)
+  (#vp:vprop)
+  (p: hpred a)
   (r:t a)
-  (h:rmem p{
-    FStar.Tactics.with_tactic selector_tactic (can_be_split p (tree_node r) /\ True)
+  (h:rmem vp{
+    FStar.Tactics.with_tactic selector_tactic (can_be_split vp (tree_node p r) /\ True)
   })
     : GTot (wdm (node a))
-  = h (tree_node r)
+  = h (tree_node p r)
 
-val reveal_non_empty_tree (#opened:inames) (#a:Type0) (ptr:t a)
-  : SteelGhost unit opened (tree_node ptr) (fun _ -> tree_node ptr)
+val reveal_non_empty_tree (#opened:inames) (#a:Type0) (p: hpred a) (ptr:t a)
+  : SteelGhost unit opened (tree_node p ptr) (fun _ -> tree_node p ptr)
              (requires fun _ -> ptr =!= null_t)
-             (ensures fun h0 _ h1 -> v_node ptr h0 == v_node ptr h1 /\
-               Spec.Node? (v_node ptr h0))
+             (ensures fun h0 _ h1 -> v_node p ptr h0 == v_node p ptr h1 /\
+               Spec.Node? (v_node p ptr h0))
 
-let reveal_non_empty_lemma (#a:Type) (ptr:t a) (t:wdm (node a)) (m:mem) : Lemma
-    (requires interp (tree_sl ptr) m /\ tree_sel_node ptr m == t /\ ptr =!= null_t)
+let reveal_non_empty_lemma (#a:Type) p (ptr:t a) (t:wdm (node a)) (m:mem) : Lemma
+    (requires interp (tree_sl p ptr) m /\ tree_sel_node p ptr m == t /\ ptr =!= null_t)
     (ensures Spec.Node? t)
-= let l' = id_elim_exists (tree_sl' ptr) m in
-  tree_sel_interp ptr l' m;
+= let l' = id_elim_exists (tree_sl' p ptr) m in
+  tree_sel_interp p ptr l' m;
   pure_interp (ptr == null_t) m
 
 let is_node (#a:Type) (t:wdm (node a)) : prop = match t with
@@ -454,10 +481,10 @@ let is_node (#a:Type) (t:wdm (node a)) : prop = match t with
   | Spec.Node _ _ _ _ _ -> True
 
 #push-options "--compat_pre_typed_indexed_effects"
-let reveal_non_empty_tree #opened #a ptr =
+let reveal_non_empty_tree #opened #a p ptr =
   let h = get () in
-  let t = hide (v_node ptr h) in
-  extract_info (tree_node ptr) t (is_node t) (reveal_non_empty_lemma ptr t)
+  let t = hide (v_node p ptr h) in
+  extract_info (tree_node p ptr) t (is_node t) (reveal_non_empty_lemma p ptr t)
 #pop-options
 
 let head (#a:Type0) (t:erased (wdm (node a)))
@@ -480,21 +507,21 @@ let gheight (#a:Type0) (t:erased (wdm (node a)))
   : Pure (erased nat) (requires Spec.Node? (reveal t)) (ensures fun _ -> True) =
   let Spec.Node _ _ _ _ h = reveal t in hide h
 
-let unpack_tree_node_lemma (#a:Type0) (pt:t a) (t:wdm (node a)) (m:mem) : Lemma
+let unpack_tree_node_lemma (#a:Type0) (p: hpred a) (pt:t a) (t:wdm (node a)) (m:mem) : Lemma
   (requires
     Spec.Node? t /\
-    interp (tree_sl pt) m /\
-    tree_sel_node pt m == t)
+    interp (tree_sl p pt) m /\
+    tree_sel_node p pt m == t)
   (ensures (
     let Spec.Node x l r s h = t in
 
     interp (ptr pt `Mem.star`
-      tree_sl (get_left x) `Mem.star`
-      tree_sl (get_right x)
+      tree_sl p (get_left x) `Mem.star`
+      tree_sl p (get_right x)
     ) m /\
     sel_of (vptr pt) m == x /\
-    tree_sel_node (get_left x) m == l /\
-    tree_sel_node (get_right x) m == r /\
+    tree_sel_node p (get_left x) m == l /\
+    tree_sel_node p (get_right x) m == r /\
     U.v (get_size x) == s /\
     U.v (get_height x) == h /\
     Spec.is_wdm l /\
@@ -502,7 +529,9 @@ let unpack_tree_node_lemma (#a:Type0) (pt:t a) (t:wdm (node a)) (m:mem) : Lemma
     s = Spec.size_of_tree t /\
     h = Spec.height_of_tree t /\
     s <= c /\
-    h <= c
+    h <= c /\
+    (G.reveal p) (get_left x) /\
+    (G.reveal p) (get_right x)
     )
   )
   =
@@ -513,11 +542,11 @@ let unpack_tree_node_lemma (#a:Type0) (pt:t a) (t:wdm (node a)) (m:mem) : Lemma
     assert (Spec.is_wds r);
     assert (Spec.is_wds t);
     assert (s == Spec.size_of_tree t);
-    tree_sel_interp pt t m;
+    tree_sel_interp p pt t m;
 
     let p1 = pts_to_sl pt full_perm x in
-    let p2 = tree_sl' (get_left x) l in
-    let p3 = tree_sl' (get_right x) r in
+    let p2 = tree_sl' p (get_left x) l in
+    let p3 = tree_sl' p (get_right x) r in
     let sl = p1 `Mem.star` p2 `Mem.star` p3 in
     assert (interp sl m);
     assert (interp (sl `Mem.star` Mem.pure (get_size x == U.uint_to_t s /\ (get_height x) == U.uint_to_t h))  m);
@@ -534,81 +563,92 @@ let unpack_tree_node_lemma (#a:Type0) (pt:t a) (t:wdm (node a)) (m:mem) : Lemma
     ptr_sel_interp pt m1;
     pts_to_witinv pt full_perm;
     // #2
-    tree_sel_interp (get_left x) l m2;
-    tree_sl'_witinv (get_left x);
+    tree_sel_interp p (get_left x) l m2;
+    tree_sl'_witinv p (get_left x);
     intro_star
       (ptr pt)
-      (tree_sl (get_left x)) m1 m2;
+      (tree_sl p (get_left x)) m1 m2;
     join_commutative m1 m2;
     assert (reveal m12 == join m1 m2);
-    assert (interp (ptr pt `Mem.star` tree_sl (get_left x)) m12);
+    assert (interp (ptr pt `Mem.star` tree_sl p (get_left x)) m12);
     // #3
-    tree_sel_interp (get_right x) r m3;
-    tree_sl'_witinv (get_right x);
+    tree_sel_interp p (get_right x) r m3;
+    tree_sl'_witinv p (get_right x);
     intro_star
-      (ptr pt `Mem.star` tree_sl (get_left x))
-      (tree_sl (get_right x)) m12 m3;
+      (ptr pt `Mem.star` tree_sl p (get_left x))
+      (tree_sl p (get_right x)) m12 m3;
     join_commutative m12 m3;
     assert (reveal m == join m12 m3);
     assert (interp (ptr pt `Mem.star`
-      tree_sl (get_left x) `Mem.star`
-      tree_sl (get_right x)
+      tree_sl p (get_left x) `Mem.star`
+      tree_sl p (get_right x)
     ) m);
 
-    Mem.pure_star_interp sl (get_size x == U.uint_to_t s /\ (get_height x) == U.uint_to_t h) m
+    Mem.pure_star_interp sl
+      (get_size x == U.uint_to_t s /\ (get_height x) == U.uint_to_t h)
+      m;
+    Mem.pure_star_interp
+      (sl `Mem.star` Mem.pure (get_size x == U.uint_to_t s /\ (get_height x) == U.uint_to_t h))
+      ((G.reveal p) (get_left x) /\ (G.reveal p) (get_right x))
+      m
 
-
-let unpack_tree_node_lemma_size (#a:Type0) (pt:t a) (t:wdm (node a)) (m:mem) : Lemma
+let unpack_tree_node_lemma_size (#a:Type0) (p: hpred a) (pt:t a) (t:wdm (node a)) (m:mem)
+  : Lemma
   (requires
     Spec.Node? t /\
-    interp (tree_sl pt) m /\
-    tree_sel_node pt m == t)
+    interp (tree_sl p pt) m /\
+    tree_sel_node p pt m == t)
   (ensures (
     reveal (gsize t) == Spec.size_of_tree t /\
     reveal (gsize t) == U.v (get_size (head t)) /\
-    reveal (gheight t) == U.v (get_height (head t))
-    )
-  )
-  = unpack_tree_node_lemma pt t m
+    reveal (gheight t) == U.v (get_height (head t)) /\
+    (G.reveal p) (get_left (head t)) /\
+    (G.reveal p) (get_right (head t))
+  ))
+  = unpack_tree_node_lemma p pt t m
 
 inline_for_extraction noextract
-let unpack_tree_node (#a:Type0) (ptr:t a)
+let unpack_tree_node (#a:Type0) (p: hpred a) (ptr:t a)
   : Steel (node a)
-             (tree_node ptr)
+             (tree_node p ptr)
              (fun n ->
                vptr ptr `star`
-               tree_node (get_left n) `star`
-               tree_node (get_right n))
+               tree_node p (get_left n) `star`
+               tree_node p (get_right n))
              (fun _ -> not (is_null_t ptr))
              (fun h0 n h1 ->
-               Spec.Node? (v_node ptr h0) /\
+               Spec.Node? (v_node p ptr h0) /\
                sel ptr h1 == n /\
-               v_node ptr h0 == Spec.Node
+               v_node p ptr h0 == Spec.Node
                  (sel ptr h1)
-                 (v_node (get_left n) h1)
-                 (v_node (get_right n) h1)
+                 (v_node p (get_left n) h1)
+                 (v_node p (get_right n) h1)
                  (U.v (get_size n))
                  (U.v (get_height n)) /\
                U.v (get_size n)
-               == Spec.size_of_tree (v_node (get_left n) h1)
-                + Spec.size_of_tree (v_node (get_right n) h1) + 1 /\
+               == Spec.size_of_tree (v_node p (get_left n) h1)
+                + Spec.size_of_tree (v_node p (get_right n) h1) + 1 /\
                U.v (get_height n)
-               == M.max (Spec.height_of_tree (v_node (get_left n) h1))
-                        (Spec.height_of_tree (v_node (get_right n) h1)) + 1 /\
+               == M.max (Spec.height_of_tree (v_node p (get_left n) h1))
+                        (Spec.height_of_tree (v_node p (get_right n) h1)) + 1 /\
                U.v (get_size n) <= c /\
-               U.v (get_height n) <= c
+               U.v (get_height n) <= c /\
+               (G.reveal p) (get_left n) /\
+               (G.reveal p) (get_right n)
              )
   =
   let h0 = get () in
-  let t = hide (v_node ptr h0) in
-  reveal_non_empty_tree ptr;
+  let t = hide (v_node p ptr h0) in
+  reveal_non_empty_tree p ptr;
 
   let gn = head t in
-  extract_info (tree_node ptr) t
+  extract_info (tree_node p ptr) t
     (reveal (gsize (reveal t)) == Spec.size_of_tree (reveal t) /\
       reveal (gsize (reveal t)) == U.v (get_size (reveal gn)) /\
-      reveal (gheight (reveal t)) == U.v (get_height (reveal gn)))
-    (fun m -> unpack_tree_node_lemma_size ptr t m);
+      reveal (gheight (reveal t)) == U.v (get_height (reveal gn)) /\
+      (G.reveal p) (get_left (reveal gn)) /\
+      (G.reveal p) (get_right (reveal gn)))
+    (fun m -> unpack_tree_node_lemma_size p ptr t m);
 
   assert (reveal (gsize (reveal t)) == Spec.size_of_tree (reveal t));
   let s = hide (Spec.size_of_tree (reveal t)) in
@@ -617,72 +657,79 @@ let unpack_tree_node (#a:Type0) (ptr:t a)
   assert (h <= c);
 
   change_slprop
-    (tree_node ptr)
+    (tree_node p ptr)
     (vptr ptr `star`
-    tree_node (get_left gn) `star`
-    tree_node (get_right gn))
+    tree_node p (get_left gn) `star`
+    tree_node p (get_right gn))
     t
     ((reveal gn, reveal (gleft t)), reveal (gright t))
-    (fun m -> unpack_tree_node_lemma ptr t m);
+    (fun m -> unpack_tree_node_lemma p ptr t m);
 
   let n = read ptr in
-  change_slprop_rel (tree_node (get_left gn)) (tree_node (get_left n)) (fun x y -> x == y) (fun _ -> ());
-  change_slprop_rel (tree_node (get_right gn)) (tree_node (get_right n)) (fun x y -> x == y) (fun _ -> ());
-
+  change_equal_slprop
+    (tree_node p (get_left gn))
+    (tree_node p (get_left n));
+  change_equal_slprop
+    (tree_node p (get_right gn))
+    (tree_node p (get_right n));
   return n
 
-let unpack_tree (#a: Type0) (ptr: t a)
+#restart-solver
+
+let unpack_tree (#a: Type0) (p: hpred a) (ptr: t a)
     : Steel (node a)
-      (linked_tree ptr)
+      (linked_tree p ptr)
       (fun node ->
         vptr ptr `star`
-        linked_tree (get_left node) `star`
-        linked_tree (get_right node))
+        linked_tree p (get_left node) `star`
+        linked_tree p (get_right node))
       (requires (fun h0 -> not (is_null_t ptr)))
       (ensures (fun h0 node h1 ->
-        v_linked_tree ptr h0 == Spec.Node
+        v_linked_tree p ptr h0 == Spec.Node
           (get_data (sel ptr h1))
-          (v_linked_tree (get_left node) h1)
-          (v_linked_tree (get_right node) h1)
+          (v_linked_tree p (get_left node) h1)
+          (v_linked_tree p (get_right node) h1)
           (U.v (get_size node))
           (U.v (get_height node)) /\
         (sel ptr h1) == node /\
         U.v (get_size node)
-        == Spec.size_of_tree (v_linked_tree (get_left node) h1)
-         + Spec.size_of_tree (v_linked_tree (get_right node) h1) + 1 /\
+        == Spec.size_of_tree (v_linked_tree p (get_left node) h1)
+         + Spec.size_of_tree (v_linked_tree p (get_right node) h1) + 1 /\
         U.v (get_size node) <= c /\
         U.v (get_height node)
-        == M.max (Spec.height_of_tree (v_linked_tree (get_left node) h1))
-                 (Spec.height_of_tree (v_linked_tree (get_right node) h1)) + 1 /\
-        U.v (get_height node) <= c
+        == M.max (Spec.height_of_tree (v_linked_tree p (get_left node) h1))
+                 (Spec.height_of_tree (v_linked_tree p (get_right node) h1)) + 1 /\
+        U.v (get_height node) <= c /\
+        (G.reveal p) (get_left node) /\
+        (G.reveal p) (get_right node)
       ))
   =
   let h0 = get() in
   change_slprop_rel
-    (linked_tree ptr)
-    (tree_node ptr)
+    (linked_tree p ptr)
+    (tree_node p ptr)
     (fun x y -> x == tree_view y)
     (fun _ -> ());
   let h1 = get () in
-  assert (v_linked_tree ptr h0 == tree_view (v_node ptr h1));
-  let n = unpack_tree_node ptr in
+  assert (v_linked_tree p ptr h0 == tree_view (v_node p ptr h1));
+  let n = unpack_tree_node p ptr in
   let h2 = get () in
 
   change_slprop_rel
-    (tree_node (get_left n))
-    (linked_tree (get_left n))
+    (tree_node p (get_left n))
+    (linked_tree p (get_left n))
     (fun x y -> tree_view x == y)
     (fun _ -> ());
   change_slprop_rel
-    (tree_node (get_right n))
-    (linked_tree (get_right n))
+    (tree_node p (get_right n))
+    (linked_tree p (get_right n))
     (fun x y -> tree_view x == y)
     (fun _ -> ());
   let h3 = get () in
-  assert (v_linked_tree (get_left n) h3 == tree_view (v_node (get_left n) h2));
-  assert (v_linked_tree (get_right n) h3 == tree_view (v_node (get_right n) h2));
-  tree_view_aux_same_size (v_node (get_left n) h2);
-  tree_view_aux_same_size (v_node (get_right n) h2);
-  tree_view_aux_same_height (v_node (get_left n) h2);
-  tree_view_aux_same_height (v_node (get_right n) h2);
+  assert (v_linked_tree p (get_left n) h3 == tree_view (v_node p (get_left n) h2));
+  assert (v_linked_tree p (get_right n) h3 == tree_view (v_node p (get_right n) h2));
+  tree_view_aux_same_size (v_node p (get_left n) h2);
+  tree_view_aux_same_size (v_node p (get_right n) h2);
+  tree_view_aux_same_height (v_node p (get_left n) h2);
+  tree_view_aux_same_height (v_node p (get_right n) h2);
   return n
