lib_avl_common/Impl.Core.fsti
@@ -21,6 +21,13 @@ val node (a: Type0) : Type0
 (** A tree is a ref to a node, themselves referencing other nodes *)
 let t (a: Type0) = ref (node a)
 
+module G = FStar.Ghost
+
+unfold
+let hpred (a: Type0) = p:G.erased (t a -> prop){
+  (G.reveal p) (null #(node a))
+}
+
 (** This type reflects the contents of a tree without the memory layout *)
 // TODO: to be replaced with MAX_UINT64
 noextract
@@ -64,134 +71,139 @@ val is_null_t (#a: Type0) (r: t a) : (b:bool{b <==> r == null_t})
 
 
 (** The separation logic proposition representing the memory layout of the tree *)
-val tree_sl (#a: Type0) (r: t a) : slprop u#1
+val tree_sl (#a: Type0) (p: hpred a) (ptr: t a) : slprop u#1
 
 (** Selector retrieving the contents of a tree in memory *)
-val tree_sel (#a: Type0) (r: t a) : selector (wdm a) (tree_sl r)
+val tree_sel (#a: Type0) (p: hpred a) (ptr: t a) : selector (wdm a) (tree_sl p ptr)
 
 [@@__steel_reduce__]
-let linked_tree' (#a: Type0) (r: t a) : vprop' = {
-  hp = tree_sl r;
+let linked_tree' (#a: Type0) (p: hpred a) (ptr: t a) : vprop' = {
+  hp = tree_sl p ptr;
   t = wdm a;
-  sel = tree_sel r
+  sel = tree_sel p ptr
 }
 
 (** The view proposition encapsulating the separation logic proposition and the selector *)
-unfold let linked_tree (#a: Type0) (tr: t a) : vprop = VUnit (linked_tree' tr)
+unfold let linked_tree (#a: Type0) (p: hpred a) (ptr: t a) : vprop = VUnit (linked_tree' p ptr)
 
 (** This convenience helper retrieves the contents of a tree from an [rmem] *)
 [@@ __steel_reduce__]
 let v_linked_tree
   (#a:Type0)
-  (#p:vprop)
-  (r:t a)
-  (h:rmem p{
-    FStar.Tactics.with_tactic selector_tactic (can_be_split p (linked_tree r) /\ True)
+  (#vp:vprop)
+  (p: hpred a)
+  (ptr:t a)
+  (h:rmem vp{
+    FStar.Tactics.with_tactic selector_tactic (can_be_split vp (linked_tree p ptr) /\ True)
   })
     : GTot (wdm a)
-  = h (linked_tree r)
+  = h (linked_tree p ptr)
 
 (*** Operations *)
 
 (**** Low-level operations on trees *)
 
-val intro_linked_tree_leaf (#opened:inames) (#a: Type0) (_: unit)
+val intro_linked_tree_leaf (#opened:inames) (#a: Type0) (p: hpred a) (_: unit)
     : SteelGhost unit
-      opened emp (fun _ -> linked_tree (null_t #a))
+      opened emp (fun _ -> linked_tree p (null_t #a))
       (requires (fun _ -> True))
-      (ensures (fun _ _ h1 -> v_linked_tree #a null_t h1 == Spec.Leaf))
+      (ensures (fun _ _ h1 -> v_linked_tree #a p null_t h1 == Spec.Leaf))
 
-val elim_linked_tree_leaf (#opened:inames) (#a: Type0) (ptr: t a)
+val elim_linked_tree_leaf (#opened:inames) (#a: Type0) (p: hpred a) (ptr: t a)
     : SteelGhost unit
-       opened (linked_tree ptr) (fun _ -> emp)
+       opened (linked_tree p ptr) (fun _ -> emp)
        (requires (fun _ -> is_null_t ptr))
        (ensures (fun h0 _ h1 ->
-         v_linked_tree ptr h0 == Spec.Leaf))
+         v_linked_tree p ptr h0 == Spec.Leaf))
 
-val null_is_leaf (#opened:inames) (#a: Type0) (ptr: t a)
+val null_is_leaf (#opened:inames) (#a: Type0) (p: hpred a) (ptr: t a)
     : SteelGhost unit
-       opened (linked_tree ptr) (fun _ -> linked_tree ptr)
+       opened (linked_tree p ptr) (fun _ -> linked_tree p ptr)
        (requires (fun _ -> is_null_t ptr))
        (ensures (fun h0 _ h1 ->
-         Spec.Leaf? (v_linked_tree ptr h0) /\
-         v_linked_tree ptr h0 == v_linked_tree ptr h1))
+         Spec.Leaf? (v_linked_tree p ptr h0) /\
+         v_linked_tree p ptr h0 == v_linked_tree p ptr h1))
 
-val leaf_is_null (#opened:inames) (#a: Type0) (ptr: t a)
+val leaf_is_null (#opened:inames) (#a: Type0) (p: hpred a) (ptr: t a)
     : SteelGhost unit
-       opened (linked_tree ptr) (fun _ -> linked_tree ptr)
-       (requires (fun h0 -> Spec.Leaf? (v_linked_tree ptr h0)))
+       opened (linked_tree p ptr) (fun _ -> linked_tree p ptr)
+       (requires (fun h0 -> Spec.Leaf? (v_linked_tree p ptr h0)))
        (ensures (fun h0 _ h1 ->
          is_null_t ptr /\
-         v_linked_tree ptr h0 == v_linked_tree ptr h1))
+         v_linked_tree p ptr h0 == v_linked_tree p ptr h1))
 
-val node_is_not_null (#opened:inames) (#a: Type0) (ptr: t a)
+val node_is_not_null (#opened:inames) (#a: Type0) (p: hpred a) (ptr: t a)
     : SteelGhost unit
-       opened (linked_tree ptr) (fun _ -> linked_tree ptr)
-       (requires (fun h0 -> Spec.Node? (v_linked_tree ptr h0)))
+       opened (linked_tree p ptr) (fun _ -> linked_tree p ptr)
+       (requires (fun h0 -> Spec.Node? (v_linked_tree p ptr h0)))
        (ensures (fun h0 _ h1 ->
          not (is_null_t ptr) /\
-         v_linked_tree ptr h0 == v_linked_tree ptr h1))
+         v_linked_tree p ptr h0 == v_linked_tree p ptr h1))
 
-val not_null_is_node (#opened:inames) (#a: Type0) (ptr: t a)
+val not_null_is_node (#opened:inames) (#a: Type0) (p: hpred a) (ptr: t a)
     : SteelGhost unit
-       opened (linked_tree ptr) (fun _ -> linked_tree ptr)
+       opened (linked_tree p ptr) (fun _ -> linked_tree p ptr)
        (requires (fun _ -> not (is_null_t ptr)))
        (ensures (fun h0 _ h1 ->
-         Spec.Node? (v_linked_tree ptr h0) /\
-         v_linked_tree ptr h0 == v_linked_tree ptr h1))
+         Spec.Node? (v_linked_tree p ptr h0) /\
+         v_linked_tree p ptr h0 == v_linked_tree p ptr h1))
 
-val pack_tree (#opened:inames) (#a: Type0)
+val pack_tree (#opened:inames) (#a: Type0) (p: hpred a)
   (ptr: t a) (left right: t a) (sr hr: U.t)
     : SteelGhost unit
       opened
       (vptr ptr `star`
-      linked_tree left `star`
-      linked_tree right)
-      (fun _ -> linked_tree ptr)
+      linked_tree p left `star`
+      linked_tree p right)
+      (fun _ -> linked_tree p ptr)
       (requires fun h0 ->
         get_left (sel ptr h0) == left /\
         get_right (sel ptr h0) == right /\
         get_size (sel ptr h0) == sr /\
         get_height (sel ptr h0) == hr /\
-        U.v sr == Spec.size_of_tree (v_linked_tree left h0) +
-                  Spec.size_of_tree (v_linked_tree right h0) +
+        U.v sr == Spec.size_of_tree (v_linked_tree p left h0) +
+                  Spec.size_of_tree (v_linked_tree p right h0) +
                   1 /\
         U.v hr == M.max
-          (Spec.height_of_tree (v_linked_tree left h0))
-          (Spec.height_of_tree (v_linked_tree right h0))
+          (Spec.height_of_tree (v_linked_tree p left h0))
+          (Spec.height_of_tree (v_linked_tree p right h0))
           + 1 /\
-        U.v sr <= c
+        U.v sr <= c /\
+        (G.reveal p) left /\
+        (G.reveal p) right
       )
       (ensures (fun h0 _ h1 ->
         let x = get_data (sel ptr h0) in
-        let l = v_linked_tree left h0 in
-        let r = v_linked_tree right h0 in
-        v_linked_tree ptr h1 == Spec.Node x l r (U.v sr) (U.v hr)))
+        let l = v_linked_tree p left h0 in
+        let r = v_linked_tree p right h0 in
+        v_linked_tree p ptr h1 == Spec.Node x l r (U.v sr) (U.v hr)))
 
 inline_for_extraction noextract
-val unpack_tree (#a: Type0) (ptr: t a)
+val unpack_tree (#a: Type0) (p: hpred a) (ptr: t a)
     : Steel (node a)
-      (linked_tree ptr)
+      (linked_tree p ptr)
       (fun node ->
         vptr ptr `star`
-        linked_tree (get_left node) `star`
-        linked_tree (get_right node))
+        linked_tree p (get_left node) `star`
+        linked_tree p (get_right node))
       (requires (fun h0 -> not (is_null_t ptr)))
       (ensures (fun h0 node h1 ->
-        v_linked_tree ptr h0 == Spec.Node
+        v_linked_tree p ptr h0 == Spec.Node
           (get_data (sel ptr h1))
-          (v_linked_tree (get_left node) h1)
-          (v_linked_tree (get_right node) h1)
+          (v_linked_tree p (get_left node) h1)
+          (v_linked_tree p (get_right node) h1)
           (U.v (get_size node))
           (U.v (get_height node))
         /\
         sel ptr h1 == node /\
         U.v (get_size node)
-        == Spec.size_of_tree (v_linked_tree (get_left node) h1)
-         + Spec.size_of_tree (v_linked_tree (get_right node) h1) + 1 /\
+        == Spec.size_of_tree (v_linked_tree p (get_left node) h1)
+         + Spec.size_of_tree (v_linked_tree p (get_right node) h1) + 1 /\
         U.v (get_height node)
-        == M.max (Spec.height_of_tree (v_linked_tree (get_left node) h1))
-                 (Spec.height_of_tree (v_linked_tree (get_right node) h1)) + 1 /\
+        == M.max (Spec.height_of_tree (v_linked_tree p (get_left node) h1))
+                 (Spec.height_of_tree (v_linked_tree p (get_right node) h1)) + 1 /\
         U.v (get_size node) <= c /\
-        U.v (get_height node) <= c
+        U.v (get_height node) <= c /\
+        (G.reveal p) (get_left node) /\
+        (G.reveal p) (get_right node)
       ))
