lib_avl_mono/Impl.AVL.M.fst
@@ -24,26 +24,26 @@ open Impl.BST.M
 //@AVL
 #push-options "--fuel 1 --ifuel 1"
 let rec is_balanced_global (ptr: t)
-  : Steel bool (linked_tree ptr) (fun _ -> linked_tree ptr)
+  : Steel bool (linked_tree p ptr) (fun _ -> linked_tree p ptr)
   (requires fun h0 -> True)
   (ensures (fun h0 b h1 ->
-      v_linked_tree ptr h0 == v_linked_tree ptr h1 /\
-      Spec.is_balanced_global (v_linked_tree ptr h0) == b))
+      v_linked_tree p ptr h0 == v_linked_tree p ptr h1 /\
+      Spec.is_balanced_global (v_linked_tree p ptr h0) == b))
   =
   if is_null_t ptr then (
-    (**) null_is_leaf ptr;
+    (**) null_is_leaf p ptr;
     return true
   ) else (
     let h = get () in
-    Spec.height_lte_size (v_linked_tree ptr h);
-    (**) let node = unpack_tree ptr in
+    Spec.height_lte_size (v_linked_tree p ptr h);
+    (**) let node = unpack_tree p ptr in
     let lh = hot_wdh (get_left node) in
     let rh = hot_wdh (get_right node) in
 
     let lbal = is_balanced_global (get_left node) in
     let rbal = is_balanced_global (get_right node) in
 
-    (**) pack_tree ptr (get_left node) (get_right node)
+    (**) pack_tree p ptr (get_left node) (get_right node)
       (get_size node) (get_height node);
     //rh + 1 >= lh
     //lh + 1 >= rh
@@ -58,23 +58,23 @@ let rec is_balanced_global (ptr: t)
 
 #push-options "--fuel 1 --ifuel 1"
 let is_balanced_local (ptr: t)
-  : Steel bool (linked_tree ptr) (fun _ -> linked_tree ptr)
+  : Steel bool (linked_tree p ptr) (fun _ -> linked_tree p ptr)
   (requires fun h0 -> True)
   (ensures (fun h0 b h1 ->
-      v_linked_tree ptr h0 == v_linked_tree ptr h1 /\
-      Spec.is_balanced_local (v_linked_tree ptr h0) == b))
+      v_linked_tree p ptr h0 == v_linked_tree p ptr h1 /\
+      Spec.is_balanced_local (v_linked_tree p ptr h0) == b))
   =
   if is_null_t ptr then (
-    (**) null_is_leaf ptr;
+    (**) null_is_leaf p ptr;
     return true
   ) else (
     let h = get () in
-    Spec.height_lte_size (v_linked_tree ptr h);
-    (**) let node = unpack_tree ptr in
+    Spec.height_lte_size (v_linked_tree p ptr h);
+    (**) let node = unpack_tree p ptr in
     let lh = hot_wdh (get_left node) in
     let rh = hot_wdh (get_right node) in
 
-    (**) pack_tree ptr (get_left node) (get_right node)
+    (**) pack_tree p ptr (get_left node) (get_right node)
       (get_size node) (get_height node);
     //rh + 1 >= lh
     //lh + 1 >= rh
@@ -90,14 +90,14 @@ let is_balanced_local (ptr: t)
 //@AVL
 #push-options "--fuel 1 --ifuel 1 --z3rlimit 100"
 let rebalance_avl (ptr: t)
-  : Steel t (linked_tree ptr) (fun ptr' -> linked_tree ptr')
+  : Steel t (linked_tree p ptr) (fun ptr' -> linked_tree p ptr')
   (requires fun h0 ->
-    Spec.Node? (v_linked_tree ptr h0)
+    Spec.Node? (v_linked_tree p ptr h0)
     ==>
-    Spec.is_avl (convert cmp) (Spec.cleft (v_linked_tree ptr h0)) /\
-    Spec.is_avl (convert cmp) (Spec.cright (v_linked_tree ptr h0)))
+    Spec.is_avl (convert cmp) (Spec.cleft (v_linked_tree p ptr h0)) /\
+    Spec.is_avl (convert cmp) (Spec.cright (v_linked_tree p ptr h0)))
   (ensures fun h0 ptr' h1 ->
-    Spec.rebalance_avl (v_linked_tree ptr h0) == v_linked_tree ptr' h1)
+    Spec.rebalance_avl (v_linked_tree p ptr h0) == v_linked_tree p ptr' h1)
     //Spec.is_avl (convert cmp) (v_linked_tree ptr' h1))
   =
   let h0 = get () in
@@ -105,93 +105,93 @@ let rebalance_avl (ptr: t)
     // TODO : fails without the assertion, why?
     // any additional line (h0, h1 or both and the assert) is enough for everything to work
     let h1 = get () in
-    assert (v_linked_tree ptr h0 == v_linked_tree ptr h1);
+    assert (v_linked_tree p ptr h0 == v_linked_tree p ptr h1);
     return ptr
   ) else (
-    Spec.not_balanced_is_not_null (v_linked_tree ptr h0);
-    assert (Spec.Node? (v_linked_tree ptr h0));
-    (**) node_is_not_null ptr;
-    (**) let node = unpack_tree ptr in
-    Spec.height_lte_size (v_linked_tree ptr h0);
+    Spec.not_balanced_is_not_null (v_linked_tree p ptr h0);
+    assert (Spec.Node? (v_linked_tree p ptr h0));
+    (**) node_is_not_null p ptr;
+    (**) let node = unpack_tree p ptr in
+    Spec.height_lte_size (v_linked_tree p ptr h0);
 
     let lh = hot_wdh (get_left node) in
     let rh = hot_wdh (get_right node) in
 
     if U.gt lh (U.add rh one) then (
 
-      (**) node_is_not_null (get_left node);
-      (**) let l_node = unpack_tree (get_left node) in
+      (**) node_is_not_null p (get_left node);
+      (**) let l_node = unpack_tree p (get_left node) in
 
       let llh = hot_wdh (get_left l_node) in
       let lrh = hot_wdh (get_right l_node) in
 
-      (**) pack_tree (get_left node) (get_left l_node) (get_right l_node)
+      (**) pack_tree p (get_left node) (get_left l_node) (get_right l_node)
         (get_size l_node) (get_height l_node);
-      (**) pack_tree ptr (get_left node) (get_right node)
+      (**) pack_tree p ptr (get_left node) (get_right node)
         (get_size node) (get_height node);
       let h = get () in
-      assert (v_linked_tree ptr h == v_linked_tree ptr h0);
-      assert (Spec.is_wdm (v_linked_tree ptr h0));
-      assert (Spec.is_wdm (Spec.cleft (v_linked_tree ptr h0)));
-      assert (Spec.is_wdm (Spec.cleft (Spec.cleft (v_linked_tree ptr h0))));
-      assert (Spec.is_wdm (Spec.cright (Spec.cleft (v_linked_tree ptr h0))));
-      assert (Spec.is_wdm (Spec.cright (v_linked_tree ptr h0)));
-      assert (U.v llh = Spec.hot_wdh (Spec.cleft (Spec.cleft (v_linked_tree ptr h0))));
-      assert (U.v lrh = Spec.hot_wdh (Spec.cright (Spec.cleft (v_linked_tree ptr h0))));
-      assert (U.v rh = Spec.hot_wdh (Spec.cright (v_linked_tree ptr h0)));
+      assert (v_linked_tree p ptr h == v_linked_tree p ptr h0);
+      assert (Spec.is_wdm (v_linked_tree p ptr h0));
+      assert (Spec.is_wdm (Spec.cleft (v_linked_tree p ptr h0)));
+      assert (Spec.is_wdm (Spec.cleft (Spec.cleft (v_linked_tree p ptr h0))));
+      assert (Spec.is_wdm (Spec.cright (Spec.cleft (v_linked_tree p ptr h0))));
+      assert (Spec.is_wdm (Spec.cright (v_linked_tree p ptr h0)));
+      assert (U.v llh = Spec.hot_wdh (Spec.cleft (Spec.cleft (v_linked_tree p ptr h0))));
+      assert (U.v lrh = Spec.hot_wdh (Spec.cright (Spec.cleft (v_linked_tree p ptr h0))));
+      assert (U.v rh = Spec.hot_wdh (Spec.cright (v_linked_tree p ptr h0)));
       assert (lh = U.add (umax llh lrh) one);
       assert (U.gt (umax llh lrh) rh);
 
       if U.gt lrh llh then (
         assert (U.gt lrh rh);
         assert (U.gte llh rh);
-        Spec.rotate_left_right_height (v_linked_tree ptr h0);
+        Spec.rotate_left_right_height (v_linked_tree p ptr h0);
         rotate_left_right ptr
 
       ) else (
         assert (U.gt llh rh);
-        Spec.rotate_right_height (v_linked_tree ptr h0);
+        Spec.rotate_right_height (v_linked_tree p ptr h0);
         rotate_right ptr
       )
 
     ) else //(
     if U.gt rh (U.add lh one) then (
 
-      (**) node_is_not_null (get_right node);
-      (**) let r_node = unpack_tree (get_right node) in
+      (**) node_is_not_null p (get_right node);
+      (**) let r_node = unpack_tree p (get_right node) in
 
       let rlh = hot_wdh (get_left r_node) in
       let rrh = hot_wdh (get_right r_node) in
 
-      (**) pack_tree (get_right node) (get_left r_node) (get_right r_node)
+      (**) pack_tree p (get_right node) (get_left r_node) (get_right r_node)
         (get_size r_node) (get_height r_node);
-      (**) pack_tree ptr (get_left node) (get_right node)
+      (**) pack_tree p ptr (get_left node) (get_right node)
         (get_size node) (get_height node);
       let h = get () in
-      assert (v_linked_tree ptr h == v_linked_tree ptr h0);
-      assert (Spec.is_wdm (Spec.cright (v_linked_tree ptr h0)));
-      assert (Spec.is_wdm (Spec.cleft (Spec.cright (v_linked_tree ptr h0))));
-      assert (Spec.is_wdm (Spec.cright (Spec.cright (v_linked_tree ptr h0))));
-      assert (Spec.is_wdm (Spec.cleft (v_linked_tree ptr h0)));
-      assert (U.v rlh = Spec.hot_wdh (Spec.cleft (Spec.cright (v_linked_tree ptr h0))));
-      assert (U.v rrh = Spec.hot_wdh (Spec.cright (Spec.cright (v_linked_tree ptr h0))));
-      assert (U.v lh = Spec.hot_wdh (Spec.cleft (v_linked_tree ptr h0)));
+      assert (v_linked_tree p ptr h == v_linked_tree p ptr h0);
+      assert (Spec.is_wdm (Spec.cright (v_linked_tree p ptr h0)));
+      assert (Spec.is_wdm (Spec.cleft (Spec.cright (v_linked_tree p ptr h0))));
+      assert (Spec.is_wdm (Spec.cright (Spec.cright (v_linked_tree p ptr h0))));
+      assert (Spec.is_wdm (Spec.cleft (v_linked_tree p ptr h0)));
+      assert (U.v rlh = Spec.hot_wdh (Spec.cleft (Spec.cright (v_linked_tree p ptr h0))));
+      assert (U.v rrh = Spec.hot_wdh (Spec.cright (Spec.cright (v_linked_tree p ptr h0))));
+      assert (U.v lh = Spec.hot_wdh (Spec.cleft (v_linked_tree p ptr h0)));
       assert (rh = U.add (umax rlh rrh) one);
       assert (U.gt (umax rlh rrh) lh);
 
       if U.gt rlh rrh then (
         assert (U.gt rlh lh);
         assert (U.gte rrh lh);
-        Spec.rotate_right_left_height (v_linked_tree ptr h0);
+        Spec.rotate_right_left_height (v_linked_tree p ptr h0);
         rotate_right_left ptr
       ) else (
         assert (U.gt rrh lh);
-        Spec.rotate_left_height (v_linked_tree ptr h0);
+        Spec.rotate_left_height (v_linked_tree p ptr h0);
         rotate_left ptr
       )
 
     ) else (
-      (**) pack_tree ptr (get_left node) (get_right node)
+      (**) pack_tree p ptr (get_left node) (get_right node)
         (get_size node) (get_height node);
       return ptr
     )
@@ -203,16 +203,16 @@ let rebalance_avl (ptr: t)
 let rec insert_avl
   (f1: f_malloc) (f2: f_free)
   (r:bool) (ptr: t) (new_data: data)
-  : Steel t (linked_tree ptr) (fun ptr' -> linked_tree ptr')
+  : Steel t (linked_tree p ptr) (fun ptr' -> linked_tree p ptr')
   (requires fun h0 ->
-    Spec.size_of_tree (v_linked_tree ptr h0) < c /\
-    Spec.height_of_tree (v_linked_tree ptr h0) < c /\
-    Spec.is_avl (convert cmp) (v_linked_tree ptr h0))
+    Spec.size_of_tree (v_linked_tree p ptr h0) < c /\
+    Spec.height_of_tree (v_linked_tree p ptr h0) < c /\
+    Spec.is_avl (convert cmp) (v_linked_tree p ptr h0))
 
   (ensures fun h0 ptr' h1 ->
-    Spec.is_avl (convert cmp) (v_linked_tree ptr h0) /\
-    Spec.insert_avl r (convert cmp) (v_linked_tree ptr h0) new_data
-    == v_linked_tree ptr' h1)
+    Spec.is_avl (convert cmp) (v_linked_tree p ptr h0) /\
+    Spec.insert_avl r (convert cmp) (v_linked_tree p ptr h0) new_data
+    == v_linked_tree p ptr' h1)
   =
   //let h0 = get () in
   //let t1 = hide (v_linked_tree ptr h0) in
@@ -230,11 +230,11 @@ let rec insert_avl
   //  <= Spec.height_of_tree t1 + 1);
 
   if is_null_t ptr then (
-    (**) null_is_leaf ptr;
-    elim_linked_tree_leaf ptr;
+    (**) null_is_leaf p ptr;
+    elim_linked_tree_leaf p ptr;
     create_tree f1 f2 new_data
   ) else (
-    (**) let node = unpack_tree ptr in
+    (**) let node = unpack_tree p ptr in
     let delta = cmp (get_data node) new_data in
     if I.eq delta szero then (
       if r then (
@@ -242,12 +242,12 @@ let rec insert_avl
           (get_left node) (get_right node)
           (get_size node) (get_height node) in
         write ptr new_node;
-        pack_tree ptr
+        pack_tree p ptr
           (get_left node) (get_right node)
           (get_size node) (get_height node);
         return ptr
       ) else (
-        pack_tree ptr
+        pack_tree p ptr
           (get_left node) (get_right node)
           (get_size node) (get_height node);
         return ptr
@@ -256,15 +256,15 @@ let rec insert_avl
       let h0 = get () in
       let new_left = insert_avl f1 f2 r (get_left node) new_data in
       let h1 = get () in
-      assert (v_linked_tree new_left h1
+      assert (v_linked_tree p new_left h1
       == Spec.insert_avl r (convert cmp)
-        (v_linked_tree (get_left node) h0) new_data);
+        (v_linked_tree p (get_left node) h0) new_data);
       Spec.insert_lemma r (convert cmp)
-        (v_linked_tree (get_left node) h0) new_data;
-      assert (Spec.size_of_tree (v_linked_tree new_left h1)
-      <= Spec.size_of_tree (v_linked_tree (get_left node) h0) + 1);
-      assert (Spec.height_of_tree (v_linked_tree new_left h1)
-      <= Spec.height_of_tree (v_linked_tree (get_left node) h0) + 1);
+        (v_linked_tree p (get_left node) h0) new_data;
+      assert (Spec.size_of_tree (v_linked_tree p new_left h1)
+      <= Spec.size_of_tree (v_linked_tree p (get_left node) h0) + 1);
+      assert (Spec.height_of_tree (v_linked_tree p new_left h1)
+      <= Spec.height_of_tree (v_linked_tree p (get_left node) h0) + 1);
       let new_ptr = merge_tree_no_alloc
         (get_data node) new_left (get_right node)
         ptr in
@@ -273,15 +273,15 @@ let rec insert_avl
       let h0 = get () in
       let new_right = insert_avl f1 f2 r (get_right node) new_data in
       let h1 = get () in
-      assert (v_linked_tree new_right h1
+      assert (v_linked_tree p new_right h1
       == Spec.insert_avl r (convert cmp)
-        (v_linked_tree (get_right node) h0) new_data);
+        (v_linked_tree p (get_right node) h0) new_data);
       Spec.insert_lemma r (convert cmp)
-        (v_linked_tree (get_right node) h0) new_data;
-      assert (Spec.size_of_tree (v_linked_tree new_right h1)
-      <= Spec.size_of_tree (v_linked_tree (get_right node) h0) + 1);
-      assert (Spec.height_of_tree (v_linked_tree new_right h1)
-      <= Spec.height_of_tree (v_linked_tree (get_right node) h0) + 1);
+        (v_linked_tree p (get_right node) h0) new_data;
+      assert (Spec.size_of_tree (v_linked_tree p new_right h1)
+      <= Spec.size_of_tree (v_linked_tree p (get_right node) h0) + 1);
+      assert (Spec.height_of_tree (v_linked_tree p new_right h1)
+      <= Spec.height_of_tree (v_linked_tree p (get_right node) h0) + 1);
       let new_ptr = merge_tree_no_alloc
         (get_data node) (get_left node) new_right
         ptr in
@@ -299,32 +299,32 @@ let rec remove_leftmost_avl
   (f1: f_malloc) (f2: f_free)
   (ptr: t)
   : Steel result
-  (linked_tree ptr)
-  (fun r -> linked_tree r.ptr)
+  (linked_tree p ptr)
+  (fun r -> linked_tree p r.ptr)
   (requires fun h0 ->
-    Spec.Node? (v_linked_tree ptr h0) /\
-    Spec.is_avl (convert cmp) (v_linked_tree ptr h0))
+    Spec.Node? (v_linked_tree p ptr h0) /\
+    Spec.is_avl (convert cmp) (v_linked_tree p ptr h0))
   (ensures fun h0 r h1 ->
-    Spec.Node? (v_linked_tree ptr h0) /\
-    Spec.is_avl (convert cmp) (v_linked_tree ptr h0) /\
-    v_linked_tree r.ptr h1
+    Spec.Node? (v_linked_tree p ptr h0) /\
+    Spec.is_avl (convert cmp) (v_linked_tree p ptr h0) /\
+    v_linked_tree p r.ptr h1
     == fst (Spec.remove_leftmost_avl
-      (convert cmp) (v_linked_tree ptr h0)) /\
+      (convert cmp) (v_linked_tree p ptr h0)) /\
     r.data == snd (Spec.remove_leftmost_avl
-      (convert cmp) (v_linked_tree ptr h0)) /\
-    Spec.size_of_tree (v_linked_tree r.ptr h1)
-    == Spec.size_of_tree (v_linked_tree ptr h0) - 1 /\
-    Spec.is_avl (convert cmp) (v_linked_tree ptr h0))
+      (convert cmp) (v_linked_tree p ptr h0)) /\
+    Spec.size_of_tree (v_linked_tree p r.ptr h1)
+    == Spec.size_of_tree (v_linked_tree p ptr h0) - 1 /\
+    Spec.is_avl (convert cmp) (v_linked_tree p ptr h0))
   =
-  (**) node_is_not_null ptr;
-  (**) let node = unpack_tree ptr in
+  (**) node_is_not_null p ptr;
+  (**) let node = unpack_tree p ptr in
   if is_null_t (get_left node) then (
     let data = get_data node in
-    elim_linked_tree_leaf (get_left node);
+    elim_linked_tree_leaf p (get_left node);
     f2 ptr;
     return {ptr = get_right node; data}
   ) else (
-    (**) not_null_is_node (get_left node);
+    (**) not_null_is_node p (get_left node);
     let r0 = remove_leftmost_avl f1 f2 (get_left node) in
     let new_ptr = merge_tree_no_alloc
       (get_data node) r0.ptr (get_right node)
@@ -347,32 +347,32 @@ let delete_avl_aux0
   (f1: f_malloc) (f2: f_free)
   (ptr: t) (data_to_rm: data)
   : Steel t
-  (linked_tree ptr)
-  (fun ptr' -> linked_tree ptr')
+  (linked_tree p ptr)
+  (fun ptr' -> linked_tree p ptr')
   (requires fun h0 ->
-    Spec.Node? (v_linked_tree ptr h0) /\
-    Spec.is_avl (convert cmp) (v_linked_tree ptr h0) /\
-    (convert cmp) (Spec.cdata (v_linked_tree ptr h0)) data_to_rm = 0)
+    Spec.Node? (v_linked_tree p ptr h0) /\
+    Spec.is_avl (convert cmp) (v_linked_tree p ptr h0) /\
+    (convert cmp) (Spec.cdata (v_linked_tree p ptr h0)) data_to_rm = 0)
   (ensures fun h0 ptr' h1 ->
-    Spec.Node? (v_linked_tree ptr h0) /\
-    Spec.is_avl (convert cmp) (v_linked_tree ptr h0) /\
-    (convert cmp) (Spec.cdata (v_linked_tree ptr h0)) data_to_rm = 0 /\
-    v_linked_tree ptr' h1
+    Spec.Node? (v_linked_tree p ptr h0) /\
+    Spec.is_avl (convert cmp) (v_linked_tree p ptr h0) /\
+    (convert cmp) (Spec.cdata (v_linked_tree p ptr h0)) data_to_rm = 0 /\
+    v_linked_tree p ptr' h1
     == Spec.delete_avl_aux0
-      (convert cmp) (v_linked_tree ptr h0) data_to_rm)
+      (convert cmp) (v_linked_tree p ptr h0) data_to_rm)
   =
-  (**) node_is_not_null ptr;
-  (**) let node = unpack_tree ptr in
+  (**) node_is_not_null p ptr;
+  (**) let node = unpack_tree p ptr in
   if is_null_t (get_right node) then (
-    elim_linked_tree_leaf (get_right node);
+    elim_linked_tree_leaf p (get_right node);
     f2 ptr;
     return (get_left node)
   ) else if is_null_t (get_left node) then (
-    elim_linked_tree_leaf (get_left node);
+    elim_linked_tree_leaf p (get_left node);
     f2 ptr;
     return (get_right node)
   ) else (
-    not_null_is_node (get_right node);
+    not_null_is_node p (get_right node);
     let r0 = remove_leftmost_avl f1 f2 (get_right node) in
     let new_ptr = merge_tree_no_alloc r0.data
       (get_left node) r0.ptr
@@ -386,22 +386,22 @@ let delete_avl_aux0
 let rec delete_avl
   (f1: f_malloc) (f2: f_free)
   (ptr: t) (data_to_rm: data)
-  : Steel t (linked_tree ptr) (fun ptr' -> linked_tree ptr')
+  : Steel t (linked_tree p ptr) (fun ptr' -> linked_tree p ptr')
   (requires fun h0 ->
-    Spec.is_avl (convert cmp) (v_linked_tree ptr h0))
+    Spec.is_avl (convert cmp) (v_linked_tree p ptr h0))
   (ensures fun h0 ptr' h1 ->
-    Spec.is_avl (convert cmp) (v_linked_tree ptr h0) /\
-    Spec.delete_avl (convert cmp) (v_linked_tree ptr h0) data_to_rm
-    == v_linked_tree ptr' h1)
+    Spec.is_avl (convert cmp) (v_linked_tree p ptr h0) /\
+    Spec.delete_avl (convert cmp) (v_linked_tree p ptr h0) data_to_rm
+    == v_linked_tree p ptr' h1)
   =
   if is_null_t ptr then (
-    (**) null_is_leaf ptr;
+    (**) null_is_leaf p ptr;
     return ptr
   ) else (
-    (**) let node = unpack_tree ptr in
+    (**) let node = unpack_tree p ptr in
     let delta = cmp data_to_rm (get_data node) in
   if I.eq delta szero then (
-    pack_tree ptr
+    pack_tree p ptr
       (get_left node) (get_right node)
       (get_size node) (get_height node);
     let ptr = delete_avl_aux0 f1 f2 ptr data_to_rm in
@@ -410,15 +410,15 @@ let rec delete_avl
     let h0 = get () in
     let new_left = delete_avl f1 f2 (get_left node) data_to_rm in
     let h1 = get () in
-    assert (v_linked_tree new_left h1
+    assert (v_linked_tree p new_left h1
     == Spec.delete_avl (convert cmp)
-      (v_linked_tree (get_left node) h0) data_to_rm);
+      (v_linked_tree p (get_left node) h0) data_to_rm);
     Spec.delete_lemma (convert cmp)
-      (v_linked_tree (get_left node) h0) data_to_rm;
-    assert (Spec.size_of_tree (v_linked_tree new_left h1)
-    <= Spec.size_of_tree (v_linked_tree (get_left node) h0));
-    assert (Spec.height_of_tree (v_linked_tree new_left h1)
-    <= Spec.height_of_tree (v_linked_tree (get_left node) h0));
+      (v_linked_tree p (get_left node) h0) data_to_rm;
+    assert (Spec.size_of_tree (v_linked_tree p new_left h1)
+    <= Spec.size_of_tree (v_linked_tree p (get_left node) h0));
+    assert (Spec.height_of_tree (v_linked_tree p new_left h1)
+    <= Spec.height_of_tree (v_linked_tree p (get_left node) h0));
     let new_ptr = merge_tree_no_alloc
       (get_data node) new_left (get_right node)
       ptr in
@@ -427,15 +427,15 @@ let rec delete_avl
     let h0 = get () in
     let new_right = delete_avl f1 f2 (get_right node) data_to_rm in
     let h1 = get () in
-    assert (v_linked_tree new_right h1
+    assert (v_linked_tree p new_right h1
     == Spec.delete_avl (convert cmp)
-      (v_linked_tree (get_right node) h0) data_to_rm);
+      (v_linked_tree p (get_right node) h0) data_to_rm);
     Spec.delete_lemma (convert cmp)
-      (v_linked_tree (get_right node) h0) data_to_rm;
-    assert (Spec.size_of_tree (v_linked_tree new_right h1)
-    <= Spec.size_of_tree (v_linked_tree (get_right node) h0));
-    assert (Spec.height_of_tree (v_linked_tree new_right h1)
-    <= Spec.height_of_tree (v_linked_tree (get_right node) h0));
+      (v_linked_tree p (get_right node) h0) data_to_rm;
+    assert (Spec.size_of_tree (v_linked_tree p new_right h1)
+    <= Spec.size_of_tree (v_linked_tree p (get_right node) h0));
+    assert (Spec.height_of_tree (v_linked_tree p new_right h1)
+    <= Spec.height_of_tree (v_linked_tree p (get_right node) h0));
     let new_ptr = merge_tree_no_alloc
       (get_data node) (get_left node) new_right
       ptr in
