lib_avl_mono/Impl.Trees.M.fst
@@ -11,6 +11,7 @@ module Spec = Spec.Trees
 module U = FStar.UInt64
 module I = FStar.Int64
 module M = FStar.Math.Lib
+module G = FStar.Ghost
 
 open Impl.Core
 open Impl.Common
@@ -18,21 +19,17 @@ open Impl.Trees.Types
 
 #set-options "--fuel 0 --ifuel 0 --ide_id_info_off"
 
-//inline_for_extraction noextract
-//let unpack_tree = unpack_tree #data
-
 //@Trees
 inline_for_extraction noextract
 let create_leaf
-  //(f1: f_malloc) (f2: f_free)
   (_:unit)
   : Steel t
-  emp (fun ptr -> linked_tree ptr)
+  emp (fun ptr -> linked_tree p ptr)
   (requires fun _ -> True)
   (ensures fun _ ptr h1 ->
-    v_linked_tree ptr h1 == Spec.Leaf)
+    v_linked_tree p ptr h1 == Spec.Leaf)
 
-  = intro_linked_tree_leaf ();
+  = intro_linked_tree_leaf p ();
     return null_t
 
 //@Trees
@@ -42,11 +39,11 @@ let create_tree
   (f1: f_malloc) (f2: f_free)
   (v: data)
   : Steel t
-  emp (fun ptr -> linked_tree ptr)
+  emp (fun ptr -> linked_tree p ptr)
   (requires fun _ -> True)
   (ensures fun _ ptr h1 ->
     not (is_null_t ptr) /\
-    v_linked_tree ptr h1 ==
+    v_linked_tree p ptr h1 ==
     Spec.Node v Spec.Leaf Spec.Leaf (U.v one) (U.v one))
   =
   let l = create_leaf () in
@@ -55,8 +52,8 @@ let create_tree
   let hr = one in
   let n = mk_node v l r sr hr in
   let ptr = f1 n in
-  pack_tree ptr l r sr hr;
-  node_is_not_null ptr;
+  pack_tree p ptr l r sr hr;
+  node_is_not_null p ptr;
   return ptr
 #pop-options
 
@@ -66,30 +63,30 @@ let sot_wds
   //(f1: f_malloc) (f2: f_free)
   (ptr: t)
   : Steel U.t
-  (linked_tree ptr)
-  (fun _ -> linked_tree ptr)
+  (linked_tree p ptr)
+  (fun _ -> linked_tree p ptr)
   (requires fun _ -> True)
   (ensures (fun h0 s h1 ->
-    v_linked_tree ptr h0 == v_linked_tree ptr h1 /\
-    U.v s == Spec.sot_wds (v_linked_tree ptr h0) /\
-    U.v s == Spec.size_of_tree (v_linked_tree ptr h0)
+    v_linked_tree p ptr h0 == v_linked_tree p ptr h1 /\
+    U.v s == Spec.sot_wds (v_linked_tree p ptr h0) /\
+    U.v s == Spec.size_of_tree (v_linked_tree p ptr h0)
   ))
   =
   if is_null_t ptr then (
     assert (is_null_t ptr);
-    null_is_leaf ptr;
+    null_is_leaf p ptr;
     let h = get () in
-    assert (0 == Spec.sot_wds (v_linked_tree ptr h));
+    assert (0 == Spec.sot_wds (v_linked_tree p ptr h));
     return zero
   ) else (
     let h1 = get () in
-    (**) let node = unpack_tree ptr in
+    (**) let node = unpack_tree p ptr in
     let h2 = get () in
-    let ptr_t1 = hide (v_linked_tree ptr h1) in
+    let ptr_t1 = hide (v_linked_tree p ptr h1) in
     let ptr_t2 = hide (Spec.Node
       (get_data (sel ptr h2))
-      (v_linked_tree (get_left node) h2)
-      (v_linked_tree (get_right node) h2)
+      (v_linked_tree p (get_left node) h2)
+      (v_linked_tree p (get_right node) h2)
       (U.v (get_size node))
       (U.v (get_height node))
     ) in
@@ -100,8 +97,8 @@ let sot_wds
     assert (reveal ptr_s1 == reveal ptr_s2);
     assert (reveal ptr_s1 == Spec.size_of_tree (reveal ptr_t1));
     let s = (get_size node) in
-    assert (U.v s == Spec.sot_wds (v_linked_tree ptr h1));
-    pack_tree ptr
+    assert (U.v s == Spec.sot_wds (v_linked_tree p ptr h1));
+    pack_tree p ptr
       (get_left node)
       (get_right node)
       (get_size node)
@@ -114,30 +111,30 @@ let hot_wdh
   //(f1: f_malloc) (f2: f_free)
   (ptr: t)
   : Steel U.t
-  (linked_tree ptr)
-  (fun _ -> linked_tree ptr)
+  (linked_tree p ptr)
+  (fun _ -> linked_tree p ptr)
   (requires fun _ -> True)
   (ensures (fun h0 h h1 ->
-    v_linked_tree ptr h0 == v_linked_tree ptr h1 /\
-    U.v h == Spec.hot_wdh (v_linked_tree ptr h0) /\
-    U.v h == Spec.height_of_tree (v_linked_tree ptr h0)
+    v_linked_tree p ptr h0 == v_linked_tree p ptr h1 /\
+    U.v h == Spec.hot_wdh (v_linked_tree p ptr h0) /\
+    U.v h == Spec.height_of_tree (v_linked_tree p ptr h0)
   ))
   =
   if is_null_t ptr then (
     assert (is_null_t ptr);
-    null_is_leaf ptr;
+    null_is_leaf p ptr;
     let h = get () in
-    assert (0 == Spec.hot_wdh (v_linked_tree ptr h));
+    assert (0 == Spec.hot_wdh (v_linked_tree p ptr h));
     return zero
   ) else (
     let h1 = get () in
-    (**) let node = unpack_tree ptr in
+    (**) let node = unpack_tree p ptr in
     let h2 = get () in
-    let ptr_t1 = hide (v_linked_tree ptr h1) in
+    let ptr_t1 = hide (v_linked_tree p ptr h1) in
     let ptr_t2 = hide (Spec.Node
       (get_data (sel ptr h2))
-      (v_linked_tree (get_left node) h2)
-      (v_linked_tree (get_right node) h2)
+      (v_linked_tree p (get_left node) h2)
+      (v_linked_tree p (get_right node) h2)
       (U.v (get_size node))
       (U.v (get_height node))
     ) in
@@ -148,8 +145,8 @@ let hot_wdh
     assert (reveal ptr_s1 == reveal ptr_s2);
     assert (reveal ptr_s1 == Spec.size_of_tree (reveal ptr_t1));
     let h = (get_height node) in
-    assert (U.v h == Spec.hot_wdh (v_linked_tree ptr h1));
-    pack_tree ptr
+    assert (U.v h == Spec.hot_wdh (v_linked_tree p ptr h1));
+    pack_tree p ptr
       (get_left node)
       (get_right node)
       (get_size node)
@@ -162,24 +159,24 @@ let merge_tree
   (f1: f_malloc) (f2: f_free)
   (v: data) (l r: t)
   : Steel t
-  (linked_tree l `star` linked_tree r)
-  (fun ptr -> linked_tree ptr)
+  (linked_tree p l `star` linked_tree p r)
+  (fun ptr -> linked_tree p ptr)
   (requires fun h0 ->
-    let sl = Spec.size_of_tree (v_linked_tree l h0) in
-    let sr = Spec.size_of_tree (v_linked_tree r h0) in
-    let hl = Spec.height_of_tree (v_linked_tree l h0) in
-    let hr = Spec.height_of_tree (v_linked_tree r h0) in
+    let sl = Spec.size_of_tree (v_linked_tree p l h0) in
+    let sr = Spec.size_of_tree (v_linked_tree p r h0) in
+    let hl = Spec.height_of_tree (v_linked_tree p l h0) in
+    let hr = Spec.height_of_tree (v_linked_tree p r h0) in
     sl + sr + 1 <= c /\
     M.max hl hr + 1 <= c)
   (ensures fun h0 ptr h1 ->
-    v_linked_tree ptr h1
+    v_linked_tree p ptr h1
     == Spec.merge_tree
       v
-      (v_linked_tree l h0)
-      (v_linked_tree r h0)
+      (v_linked_tree p l h0)
+      (v_linked_tree p r h0)
     /\
-    Spec.csize (v_linked_tree ptr h1) <= c /\
-    Spec.cheight (v_linked_tree ptr h1) <= c)
+    Spec.csize (v_linked_tree p ptr h1) <= c /\
+    Spec.cheight (v_linked_tree p ptr h1) <= c)
   =
   let s1 = sot_wds l in
   let s2 = sot_wds r in
@@ -189,33 +186,36 @@ let merge_tree
   let h = U.add (umax h1 h2) one in
   let n = mk_node v l r s h in
   let ptr = f1 n in
-  pack_tree ptr l r s h;
+  pack_tree p ptr l r s h;
   return ptr
 
 inline_for_extraction noextract
 let merge_tree_no_alloc
   (v: data) (l r: t) (ptr: ref node)
   : Steel t
-  (linked_tree l `star`
-  linked_tree r `star`
+  (linked_tree p l `star`
+  linked_tree p r `star`
   vptr ptr)
-  (fun ptr' -> linked_tree ptr')
+  (fun ptr' -> linked_tree p ptr')
   (requires fun h0 ->
-    let sl = Spec.size_of_tree (v_linked_tree l h0) in
-    let sr = Spec.size_of_tree (v_linked_tree r h0) in
-    let hl = Spec.height_of_tree (v_linked_tree l h0) in
-    let hr = Spec.height_of_tree (v_linked_tree r h0) in
+    let sl = Spec.size_of_tree (v_linked_tree p l h0) in
+    let sr = Spec.size_of_tree (v_linked_tree p r h0) in
+    let hl = Spec.height_of_tree (v_linked_tree p l h0) in
+    let hr = Spec.height_of_tree (v_linked_tree p r h0) in
     sl + sr + 1 <= c /\
-    M.max hl hr + 1 <= c)
+    M.max hl hr + 1 <= c /\
+    (G.reveal p) l /\
+    (G.reveal p) r
+  )
   (ensures fun h0 ptr' h1 ->
-    v_linked_tree ptr' h1
+    v_linked_tree p ptr' h1
     == Spec.merge_tree
       v
-      (v_linked_tree l h0)
-      (v_linked_tree r h0)
+      (v_linked_tree p l h0)
+      (v_linked_tree p r h0)
     /\
-    Spec.csize (v_linked_tree ptr' h1) <= c /\
-    Spec.cheight (v_linked_tree ptr' h1) <= c)
+    Spec.csize (v_linked_tree p ptr' h1) <= c /\
+    Spec.cheight (v_linked_tree p ptr' h1) <= c)
   =
   let s1 = sot_wds l in
   let s2 = sot_wds r in
@@ -225,5 +225,5 @@ let merge_tree_no_alloc
   let h = U.add (umax h1 h2) one in
   let n = mk_node v l r s h in
   write ptr n;
-  pack_tree ptr l r s h;
+  pack_tree p ptr l r s h;
   return ptr
