lib_avl_mono/Impl.Trees.Types.fst
@@ -9,6 +9,7 @@ open Impl.Core
 
 module US = FStar.SizeT
 module U64 = FStar.UInt64
+module U32 = FStar.UInt32
 module U8 = FStar.UInt8
 module I64 = FStar.Int64
 
@@ -16,6 +17,72 @@ noextract inline_for_extraction
 let array = Steel.ST.Array.array
 
 open Config
+open Utils2
+
+assume val avl_data_size_aux : v:U32.t{U32.v v <= U32.v page_size}
+
+let avl_data_size : sc =
+  if U32.lte avl_data_size_aux 64ul then 64ul else avl_data_size_aux
+
+open SizeClass
+open Main
+
+inline_for_extraction noextract
+val init_avl_scs (slab_region: array U8.t)
+  : Steel (size_class_struct)
+  (A.varray slab_region)
+  (fun r -> size_class_vprop r)
+  (requires fun h0 ->
+    A.length slab_region = US.v metadata_max `FStar.Mul.op_Star` U32.v Config.page_size /\
+    zf_u8 (A.asel slab_region h0)
+  )
+  (ensures fun _ r _ ->
+    r.size = avl_data_size /\
+    r.slab_region == slab_region
+  )
+
+let init_avl_scs (slab_region: array U8.t)
+  =
+  let md_bm_region_size = US.mul metadata_max 4sz in
+  let md_region_size = metadata_max in
+  let md_bm_region = mmap_u64 md_bm_region_size in
+  let md_region = mmap_cell_status md_region_size in
+  let scs = init_struct_aux avl_data_size slab_region md_bm_region md_region in
+  return scs
+
+module L = Steel.SpinLock
+
+noeq
+type mmap_md_slabs =
+  {
+    slab_region: array U8.t;
+    scs: v:size_class_struct{
+      v.size = avl_data_size /\
+      v.slab_region == A.split_r slab_region 0sz
+    };
+    lock : L.lock (
+      size_class_vprop scs `star`
+      A.varray (A.split_l slab_region 0sz)
+    );
+  }
+
+let init_mmap_md_slabs (_:unit)
+  : SteelTop mmap_md_slabs false (fun _ -> emp) (fun _ _ _ -> True)
+  =
+  let slab_region_size = US.mul metadata_max (US.uint32_to_sizet Config.page_size) in
+  let slab_region = mmap_u8 slab_region_size in
+  A.ghost_split slab_region 0sz;
+  let scs = init_avl_scs (A.split_r slab_region 0sz) in
+  let lock = L.new_lock (size_class_vprop scs `star` A.varray (A.split_l slab_region 0sz)) in
+  return { slab_region; scs; lock; }
+
+// intentional top-level effect for initialization
+// corresponding warning temporarily disabled
+#push-options "--warn_error '-272'"
+let metadata_slabs : mmap_md_slabs = init_mmap_md_slabs ()
+#pop-options
+
+#restart-solver
 
 type data = x: (array U8.t * US.t){
   (
@@ -30,12 +97,64 @@ type data = x: (array U8.t * US.t){
   US.v (snd x) == 0
 }
 
-let node = node data
-let t = t data
+//TODO: discussion with Aymeric and Jonathan
+//generalizing the slabs allocator type should allow
+//to remove this cast
+//but polymorphic assumes are unsupported
+//pass corresponding mmap function (which is the needed one)
+//as argument to avoid this issue
 
-//TO BE REMOVED
-//noextract
-//assume val ptr_to_u64 (x: array U8.t) : U64.t
+let node = node data
+
+assume val array_u8__to__ref_node
+  (arr: array U8.t)
+  : Steel (ref node)
+  (A.varray arr)
+  (fun r -> vptr r)
+  (requires fun _ -> A.length arr == U32.v avl_data_size)
+  (ensures fun _ r _ ->
+    A.is_null arr = is_null r
+  )
+
+assume val ref_node__to__array_u8_tot
+  (x: ref node)
+  : Pure (array U8.t)
+  (requires True)
+  (ensures fun r ->
+    A.is_null r = is_null x /\
+    A.length r == U32.v avl_data_size
+  )
+
+module UP = FStar.PtrdiffT
+
+module G = FStar.Ghost
+
+#push-options "--fuel 0 --ifuel 0"
+let p : hpred data
+  =
+  G.hide (fun (x: ref node) ->
+    let ptr = ref_node__to__array_u8_tot x in
+    is_null x \/
+    (same_base_array ptr metadata_slabs.scs.slab_region /\
+    UP.fits (A.offset (A.ptr_of ptr) - A.offset (A.ptr_of metadata_slabs.scs.slab_region)) /\
+    A.offset (A.ptr_of ptr) - A.offset (A.ptr_of metadata_slabs.scs.slab_region) >= 0 /\
+    ((A.offset (A.ptr_of ptr) - A.offset (A.ptr_of metadata_slabs.scs.slab_region)) % U32.v page_size) % U32.v metadata_slabs.scs.size = 0)
+  )
+#pop-options
+
+assume val ref_node__to__array_u8
+  (x: ref node)
+  : Steel (array U8.t)
+  (vptr x)
+  (fun r -> A.varray r)
+  (requires fun _ -> True)
+  (ensures fun _ r _ ->
+    A.is_null r = is_null x /\
+    A.length r == U32.v avl_data_size /\
+    r == ref_node__to__array_u8_tot x
+  )
+
+let t = t data
 
 // CAUTION:
 // the refinement implies that the injectivity
@@ -55,10 +174,17 @@ unfold type f_malloc
   = (x: node) -> Steel (ref node)
   emp (fun r -> vptr r)
   (requires fun _ -> True)
-  (ensures fun _ r h1 -> sel r h1 == x /\ not (is_null r))
+  (ensures fun _ r h1 ->
+    sel r h1 == x /\
+    not (is_null r) /\
+    (G.reveal p) r
+  )
 
 unfold type f_free
   = (r: ref node) -> Steel unit
-  (vptr r) (fun _ -> emp)
-  (requires fun _ -> True)
+  (vptr r)
+  (fun _ -> emp)
+  (requires fun _ ->
+    (G.reveal p) r
+  )
   (ensures fun _ _ _-> True)
