lib_avl_mono/Impl.Trees.Rotate.M.fst
@@ -23,28 +23,27 @@ open Impl.Trees.M
 #push-options "--fuel 1 --ifuel 1 --z3rlimit 25"
 let rotate_left (ptr: t)
   : Steel t
-  (linked_tree ptr)
-  (fun ptr' -> linked_tree ptr')
+  (linked_tree p ptr)
+  (fun ptr' -> linked_tree p ptr')
   (requires (fun h0 ->
-    let t = v_linked_tree ptr h0 in
+    let t = v_linked_tree p ptr h0 in
     let r = rotate_left t in
     Some? r /\
     height_of_tree (Some?.v r) <= height_of_tree t
   ))
-
   (ensures (fun h0 ptr' h1 ->
-    rotate_left (v_linked_tree ptr h0)
-    == Some (v_linked_tree ptr' h1)
+    rotate_left (v_linked_tree p ptr h0)
+    == Some (v_linked_tree p ptr' h1)
   ))
   =
   let h = get () in
-  assert (size_of_tree (v_linked_tree ptr h) <= c);
-  rotate_left_size (v_linked_tree ptr h);
-  (**) node_is_not_null ptr;
-  (**) let x_node = unpack_tree ptr in
+  assert (size_of_tree (v_linked_tree p ptr h) <= c);
+  rotate_left_size (v_linked_tree p ptr h);
+  (**) node_is_not_null p ptr;
+  (**) let x_node = unpack_tree p ptr in
   let x = get_data x_node in
-  (**) node_is_not_null (get_right x_node);
-  (**) let z_node = unpack_tree (get_right x_node) in
+  (**) node_is_not_null p (get_right x_node);
+  (**) let z_node = unpack_tree p (get_right x_node) in
   let z = get_data z_node in
 
   let new_subnode = merge_tree_no_alloc x
@@ -59,27 +58,27 @@ let rotate_left (ptr: t)
 #push-options "--fuel 1 --ifuel 1 --z3rlimit 25"
 let rotate_right (ptr: t)
   : Steel t
-  (linked_tree ptr)
-  (fun ptr' -> linked_tree ptr')
+  (linked_tree p ptr)
+  (fun ptr' -> linked_tree p ptr')
   (requires (fun h0 ->
-    let t = v_linked_tree ptr h0 in
+    let t = v_linked_tree p ptr h0 in
     let r = rotate_right t in
     Some? r /\
     height_of_tree (Some?.v r) <= height_of_tree t
   ))
   (ensures (fun h0 ptr' h1 ->
-    rotate_right (v_linked_tree ptr h0)
-    == Some (v_linked_tree ptr' h1)
+    rotate_right (v_linked_tree p ptr h0)
+    == Some (v_linked_tree p ptr' h1)
   ))
   =
   let h = get () in
-  assert (size_of_tree (v_linked_tree ptr h) <= c);
-  rotate_right_size (v_linked_tree ptr h);
-  (**) node_is_not_null ptr;
-  (**) let x_node = unpack_tree ptr in
+  assert (size_of_tree (v_linked_tree p ptr h) <= c);
+  rotate_right_size (v_linked_tree p ptr h);
+  (**) node_is_not_null p ptr;
+  (**) let x_node = unpack_tree p ptr in
   let x = get_data x_node in
-  (**) node_is_not_null (get_left x_node);
-  let z_node = unpack_tree (get_left x_node) in
+  (**) node_is_not_null p (get_left x_node);
+  let z_node = unpack_tree p (get_left x_node) in
   let z = get_data z_node in
 
   let new_subnode = merge_tree_no_alloc x
